SSA/Projects/CIRCT/Stream/Stream.lean
@@ -1,5 +1,6 @@
 import Mathlib.Data.Stream.Defs
 import Batteries.Data.List.Basic
+import SSA.Core.HVector
 
 /-!
 
@@ -16,6 +17,9 @@ Note that semantics of `DC` and `Handshake` are deterministic -/
 def Stream (β : Type) := Stream' (Option β)
 
 namespace Stream
+
+def map {α β : Type} (s : Stream α) (f : α → β) : Stream β :=
+  fun i => (s i).map f
 
 def corec {α} {β} (s0 : β) (f : β → (Option α × β)) : Stream α :=
   Stream'.corec (f · |>.fst) (f · |>.snd) s0
@@ -44,3 +48,27 @@ def ofList (vals : List α) : Stream α :=
 /-- `toList n x` returns the first `n` messages (including `none`s) as a list -/
 def toList (n : Nat) (x : Stream α) : List (Option α) :=
   List.ofFn (fun (i : Fin n) => x i)
+
+-- β such that A a = Stream β
+def transpose {A} {as : List α} (xs : HVector A as)
+    {B : α → Type}
+    (h : ∀ {a : α}, A a = Stream (B a)) :
+    Stream (HVector B as) :=
+  corec xs fun xs =>
+    -- map the vector of streams (input) to streams where the first none have been removed
+    -- e.g. f ~ popFirstNone
+    -- then, we foldl over this new vector of streams (monadic map???? the side effect is returning a `none`)
+    let xs' := xs.map fun a x =>
+      let x : Stream (B a) := cast h x
+      if x.head.isNone then
+        x.tail
+      else
+        x
+
+    let out := xs'.mapM' fun a x => x.head
+    (cast (by congr; sorry) out,
+     xs'.map fun a x => h ▸ x)
+    -- use the state of the corec to remember what elements we know/have already and what not
+    -- match as, xs with
+    -- | [], _ => corec () fun _ => (none, ())
+    -- | _::_, x ::ₕ xs => _
